backend/CleanupLabelsproof.v
@@ -274,7 +274,7 @@ Proof.
   econstructor; eauto.
 (* Lbuiltin *)
   left; econstructor; split.
-  econstructor.
+  econstructor. eauto.
   eapply eval_builtin_args_preserved with (ge1 := ge); eauto. exact symbols_preserved.
   eapply external_call_symbols_preserved; eauto. apply senv_preserved.
   eauto.
