backend/Mach.v
@@ -352,10 +352,11 @@ Inductive step: state -> trace -> state -> Prop :=
       step (State s fb (Vptr stk soff) (Mtailcall sig ros :: c) rs m)
         E0 (Callstate s f' rs m')
   | exec_Mbuiltin:
-      forall s f sp rs m ef args res b vargs t vres rs' m',
-      eval_builtin_args ge rs sp m args vargs ->
+      forall s f sp rs m ef args res b vargs t vres rs1 rs' m',
+      rs1 = undef_regs (destroyed_before_builtin ef) rs ->
+      eval_builtin_args ge rs1 sp m args vargs ->
       external_call ef ge vargs m t vres m' ->
-      rs' = set_res res vres (undef_regs (destroyed_by_builtin ef) rs) ->
+      rs' = set_res res vres (undef_regs (destroyed_during_builtin ef) rs1) ->
       step (State s f sp (Mbuiltin ef args res :: b) rs m)
          t (State s f sp b rs' m')
   | exec_Mgoto:
