x86/Asmgenproof.v
@@ -674,12 +674,16 @@ Opaque loadind.
   inv AT. monadInv H4.
   exploit functions_transl; eauto. intro FN.
   generalize (transf_function_no_overflow _ _ H3); intro NOOV.
-  exploit builtin_args_match; eauto. intros [vargs' [P Q]].
+  exploit builtin_args_match.
+    eapply agree_undef_regs with (rl := destroyed_before_builtin ef); eauto. 
+    eauto. eauto.
+  intros [vargs' [P Q]].
   exploit external_call_mem_extends; eauto.
   intros [vres' [m2' [A [B [C D]]]]].
   left. econstructor; split. apply plus_one.
   eapply exec_step_builtin. eauto. eauto.
   eapply find_instr_tail; eauto.
+  eauto.
   erewrite <- sp_val by eauto.
   eapply eval_builtin_args_preserved with (ge1 := ge); eauto. exact symbols_preserved.
   eapply external_call_symbols_preserved; eauto. apply senv_preserved.
@@ -688,13 +692,13 @@ Opaque loadind.
   instantiate (2 := tf); instantiate (1 := x).
   unfold nextinstr_nf, nextinstr. rewrite Pregmap.gss.
   rewrite undef_regs_other. rewrite set_res_other. rewrite undef_regs_other_2.
-  rewrite <- H1. simpl. econstructor; eauto.
+  rewrite <- H. simpl. econstructor; eauto.
   eapply code_tail_next_int; eauto.
   rewrite preg_notin_charact. intros. auto with asmgen.
   auto with asmgen.
   simpl; intros. intuition congruence.
   apply agree_nextinstr_nf. eapply agree_set_res; auto.
-  eapply agree_undef_regs; eauto. intros; apply undef_regs_other_2; auto.
+  eauto using agree_undef_regs, undef_regs_other_2.
   congruence.
 
 - (* Mgoto *)
